Juvix/Core/Main/Language/Value.lean
@@ -5,7 +5,7 @@ namespace Juvix.Core.Main
 
 inductive Value : Type where
   | const : Constant → Value
-  | constr_app : (constr : Name) → (args : List Value) → Value
+  | constr_app : (constr : Name) → (args_rev : List Value) → Value
   | closure : (ctx : List Value) → (value : Expr) → Value
   | unit : Value
   deriving Inhabited
